Little fixes in setoid_rewrite. - More meaningful argument name for resolve_typeclasses. - Try to remove unneeded instance declarations in Morphisms. - Allow the proofs of reflexivity arising from unchanged arguments in setoid_rewrite to be fullfiled by Morphism instances and not necessariy because the relation is reflexive (needed by higher-order morphisms). Use a new "MorphismProxy" class to implement that efficiently. - Fix a bug in abstract_generalize not delta-reducing a type where it should.
git-svn-id: svn+ssh://scm.gforge.inria.fr/svn/coq/trunk@10807 85f007b7-540e-0410-9357-904b9bb8a0f7

contrib/subtac/subtac_classes.ml
@@ -158,7 +158,7 @@ let new_instance ?(global=false) ctx (instid, bk, cl) props ?(on_free_vars=Class
   let env' = Classes.push_named_context ctx' env in
   isevars := Evarutil.nf_evar_defs !isevars;
   let sigma = Evd.evars_of !isevars in
-  isevars := resolve_typeclasses ~onlyargs:false ~all:true env' sigma !isevars;
+  isevars := resolve_typeclasses ~onlyargs:false ~fail:true env' sigma !isevars;
   let sigma = Evd.evars_of !isevars in
   let substctx = Typeclasses.nf_substitution sigma subst in
   let subst, _propsctx = 
