pretyping/typeclasses.mli
@@ -74,7 +74,7 @@ val bool_out : Dyn.t -> bool
 val is_resolvable : evar_info -> bool
 val mark_unresolvable : evar_info -> evar_info
 
-val resolve_typeclasses : ?onlyargs:bool -> ?all:bool -> env -> evar_map -> evar_defs -> evar_defs
+val resolve_typeclasses : ?onlyargs:bool -> ?fail:bool -> env -> evar_map -> evar_defs -> evar_defs
 
 val solve_instanciation_problem : (env -> evar_defs -> existential_key -> evar_info -> evar_defs * bool) ref
 val solve_instanciations_problem : (env -> evar_defs -> bool -> bool -> evar_defs) ref
